Breadth-First Reconstruction is a generalization of BFN where we give the list that should decorate nodes
BFN t = BFR t l with l = [0,...,n-1] and n = m_bt t

bfr_fifo_3q_full.v
@@ -21,256 +21,116 @@ Require Import list_utils wf_utils bt bft fifo.
 
 Set Implicit Arguments.
 
-Section seq_an.
-
-  (* seq_an a n = [a;a+1;...;a+(n-1)] *)
-
-  Fixpoint seq_an a n : list nat :=
-    match n with
-      | 0    => nil
-      | S n  => a::seq_an (S a) n
-    end.
-
-  Fact seq_an_length a n : length (seq_an a n) = n.
-  Proof. revert a; induction n; simpl; intros; f_equal; auto. Qed.
-
-  Fact seq_an_spec a n x : In x (seq_an a n) <-> a <= x < a+n.
-  Proof. 
-    revert x a; induction n as [ | n IHn ]; intros x a; simpl;
-      [ | rewrite IHn ]; omega.
-  Qed.
-
-  Fixpoint is_seq_from n (l : list nat) { struct l }: Prop :=
-    match l with  
-      | nil  => True
-      | x::l => n = x /\ is_seq_from (S n) l
-    end.
-
-  Theorem is_seq_from_spec a l : is_seq_from a l <-> exists n, l = seq_an a n.
-  Proof.
-    revert a; induction l as [ | x l IH ]; intros a; simpl.
-    + split; auto; exists 0; auto.
-    + rewrite IH; split.
-      * intros (? & n & Hn); subst x; exists (S n); subst; auto.
-      * intros ([ | n ] & ?); subst; try discriminate.
-        simpl in H; inversion H; subst; split; auto.
-        exists n; auto.
-  Qed.
-
-End seq_an.
-
-Section bfn.
+Section bfr_3q.
 
   Let fifo_3q_sum { X } (q : fifo_3q (bt X)) := lsum (fifo_3q_list q). 
 
-  Variable (X : Type).
+  Variable (X Y : Type).
 
-  Notation fX := (fifo_3q (bt X)). 
-  Notation fN := (fifo_3q (bt nat)).
+  Notation fX := (fifo_3q (bt X)).
+  Notation fY := (fifo_3q (bt Y)).
 
-  (* the forest (list of bt nat) is a breadth first numbering from n if
-     its breadth first traversal yields [n;n+1;....;m[ for some m
-   *)
-
-(*
-  Let fX_spec := fifo_3q_spec (bt X).
-  Let fN_spec := fifo_3q_spec (bt nat).
-
-*)
-
-  Definition is_bfn_from n l := is_seq_from n (bft_f l).
-
-  (* Breath First Numbering: maps a forest X to a forest nat such that
-          1) the two forests are of the same shape
-          2) the result is a breadth first numbering from n
-
-     Beware that the output is a reversed queue compared to the input
-   *)
-
-  (** We decompose the proof into Computational Content (CC) and 
-      Proof Obligations (PO) using the handy refine tactic leaving 
-      holes for PO which are thus postponed after CC.
-
-      The intended extraction is:
-
-      let rec bfn_f n p =
-        if q_void p then q_nil
-        else let c,p1 = fifo_3q_deq p 
-             in match c with
-               | Leaf _
-              -> q_enq (bfn_f (1+n) p1) (Leaf u)
-               | Node (a, _, b)
-              -> let u,q1 = q_deq (bfn_f (1+n) (q_enq (q_enq p1 a) b))     in
-                 let v,q2 = q_deq q1 
-                 in q_enq q2 (Node (v, n, u))
-
-      Hence the CC should be something like 
-
-      refine (
-        let (b,Hb) := fifo_3q_void_full p 
-        in match b with 
-          | true  
-          => let (q,Hq) := @fifo_3q_nil _
-             in exist _ q _
-          | false 
-          => let (d1,Hd1) := fifo_3q_deq_full p _ 
-             in match d1 with
-               | (leaf x    , p1) 
-               => let (q,Hq) := bfn_3q_f (S n) p1 _          in
-                  let (q1,Hq1) := fifo_3q_enq_full q (leaf n) 
-                  in exist _ q1 _
-               | (node a x b, p1) => fun Hp1 
-               => let (p2,Hp2)     := fifo_3q_enq_full p1 a    in
-                  let (p3,Hp3)     := fifo_3q_enq_full p2 b    in
-                  let (q,Hq)       := bfn_3q_f (S n) p3 _      in
-                  let ((u,q1),Hq1) := fifo_3q_deq_full q _     in
-                  let ((v,q2),Hq2) := fifo_3q_deq_full q1 _    in
-                  let (q3,Hq3)     := fifo_3q_enq_full q2 (node v n u)
-                  in  exist _ q3 _
-             end
-        end)
-
-      But this does not work well because for instance the b in Hb is
-      not decomposed into either true or false with the subsequent 
-      match b with ... end. We need to implement some kind of dependent
-      pattern matching which involves a more subtle approach
-
-      The structure of this proof is the following:
-
-      We use a series of refine to specify the CC and PO is  
-      postponed after the full CC is given using cycle tactics
-      to reorder goals and to keep CC goals upfront.
-
-      At some point, we need pattern matching to decompose 
-      term in hypotheses as well as in the conclusion. The
-      simplest way to do it is to revert the hypothesis in 
-      the conclusion before the match and then intro it in 
-      the different match branches where the matched term 
-      has been decomposed. This corresponds to dependent
-      pattern-matching but hand-writting dependent pattern-
-      matching in refines is much more complicated/verbose 
-      than just
-
-      revert Hq; refine (match q with ... => ... end); intros Hq
-
-      By postponing PO, we let the CC to develop itself in the 
-      first branch
-
-      Also, using fully specified terms like fifo_3q_enq_full 
-      instead of the pair fifo_3q_enq/fifo_3q_enq_spec allows
-      use to avoid generalizing fifo_3q_enq_spec before the
-      next pattern matching.
-
-    *)
-
-  Definition bfn_3q_f n (p : fX) : { q : fN | fifo_3q_list p ~lt rev (fifo_3q_list q) /\ is_bfn_from n (rev (fifo_3q_list q)) }.
+  Definition bfr_3q_f (p : fX) (ll : list Y) : 
+            fifo_3q_sum p = length ll
+         -> { q : fY | fifo_3q_list p ~lt rev (fifo_3q_list q) 
+                    /\ bft_f (rev (fifo_3q_list q)) = ll }.
   Proof.
-    induction on n p as bfn_3q_f with measure (fifo_3q_sum p).
+    induction on p ll as bfr_3q_f with measure (fifo_3q_sum p).
 
     refine (let (b,Hb) := fifo_3q_void_full p in _).
-    revert Hb; refine (match b with 
-      | true  => fun Hp 
-      => let (q,Hq) := @fifo_3q_nil_full _ 
-         in exist _ q _
-      | false => fun Hp 
-      => let (d1,Hd1) := fifo_3q_deq_full p _ 
-         in _
-    end). 
-    all: cycle 2. (* We queue 2 POs *)
-    revert Hd1; refine (match d1 with
-      | (leaf x    , p1) => fun Hp1 
-      => let (q,Hq)   := bfn_3q_f (S n) p1 _ in  
-         let (q1,Hq1) := fifo_3q_enq_full q (leaf n) 
-         in exist _ q1 _
-      | (node a x b, p1) => fun Hp1 
-      => let (p2,Hp2) := fifo_3q_enq_full p1 a    in
-         let (p3,Hp3) := fifo_3q_enq_full p2 b    in
-         let (q,Hq)   := bfn_3q_f (S n) p3 _ in
-         let (d2,Hd2) := fifo_3q_deq_full q _ 
-         in  _
-    end); simpl in Hp1.
-    all: cycle 4. (* We queue 4 POs *)
-    revert Hd2; refine (match d2 with (u,q1) => _ end); intros Hq1.
-    refine (let (d3,Hd3) := fifo_3q_deq_full q1 _ in _).
-    all: cycle 1. (* We queue 1 PO *) 
-    revert Hd3; refine (match d3 with 
-      | (v,q2) => fun Hq2 
-      => let (q3,Hq3) := fifo_3q_enq_full q2 (node v n u)
-         in  exist _ q3 _
-    end); simpl in Hq2, Hq3.
-    all: cycle 1. (* We queue 1 PO *) 
-
-    (* And now, we show POs *)
-   
-    * apply proj1 in Hp; rewrite Hp, Hq; split; simpl; auto.
-      red; rewrite bft_f_fix_0; simpl; auto.
-    * intros H; apply Hp in H; discriminate.
-    * unfold fifo_3q_sum; rewrite Hp1; simpl; omega.
-    * destruct Hq as (H5 & H6).
-      rewrite Hp1, Hq1.
-      subst; split; auto.
-      + rewrite rev_app_distr; simpl; auto.
-      + rewrite rev_app_distr; simpl; red.
-        rewrite bft_f_fix_3; simpl; rewrite <- app_nil_end; auto.
-    * unfold fifo_3q_sum. 
-      rewrite Hp3, Hp2, app_ass; simpl.
-      rewrite lsum_app, Hp1; simpl; omega.
-    * apply proj1, Forall2_rev in Hq; intros H; revert Hq.
-      rewrite H, Hp3, Hp2, app_ass; simpl.
-      rewrite rev_app_distr; simpl.
-      intros G; apply Forall2_length in G; discriminate.
-    * apply proj1, Forall2_rev in Hq; intros H; revert Hq.
-      rewrite Hq1, H, Hp3, Hp2, app_ass; simpl.
-      rewrite rev_app_distr; simpl.
-      intros G; apply Forall2_length in G; discriminate.
-    * destruct Hq as (H5,H6).
-      rewrite Hp3, Hp2, Hq1, Hq2 in H5. 
-      repeat (rewrite app_ass in H5; simpl in H5).
-      apply Forall2_2snoc_inv in H5.
-      destruct H5 as (G1 & G2 & H5).
-      rewrite Hq1, Hq2 in H6; simpl in H6; rewrite app_ass in H6; simpl in H6.
-      unfold is_bfn_from in H6 |- *.
+    revert b Hb; intros [|] Hb Hll.
+    { refine(let (q,Hq) := @fifo_3q_nil_full _ in exist _ q _).
+      apply proj1 in Hb; rewrite Hq.
+      unfold fifo_3q_sum in Hll.
+      rewrite Hb in Hll |- *; auto.
+      destruct ll; simpl; try discriminate.
+      rewrite bft_f_fix_0; auto. }
+    refine (let (d1,Hd1) := fifo_3q_deq_full p _ in _).
+    { red; rewrite <- Hb; discriminate. }
+    revert d1 Hd1; intros (x,p1) Hp1.
+    unfold fifo_3q_sum in Hll; rewrite Hp1 in Hll.
+    revert ll Hll; intros [ | y ll ] Hll.
+    { exfalso; simpl in Hll; generalize (m_bt_ge_1 x); omega. }
+    simpl in Hll.
+    destruct x as [ x | a x b ]. 
+    + refine (let (q,Hq) := bfr_3q_f p1 ll _ _ in _); auto.
+      { unfold fifo_3q_sum; rewrite Hp1; simpl; omega. }
+      destruct Hq as (Hq1 & Hq2).
+      refine (let (q1,Hq1) := fifo_3q_enq_full q (leaf y) in exist _ q1 _).
+      rewrite Hp1, Hq1, rev_app_distr; split; simpl; auto.
+      rewrite bft_f_fix_3, <-app_nil_end, Hq2; auto.
+    + refine (let (p2,Hp2) := fifo_3q_enq_full p1 a    in
+              let (p3,Hp3) := fifo_3q_enq_full p2 b    in
+              let (q,Hq)   := bfr_3q_f p3 ll _ _
+              in _).
+      { unfold fifo_3q_sum; rewrite Hp3, Hp2, Hp1.
+        repeat rewrite lsum_app; simpl; omega. }
+      { unfold fifo_3q_sum; rewrite Hp3, Hp2.
+        repeat rewrite lsum_app; simpl in Hll |- *; omega. }
+      destruct Hq as (Hq_1 & Hq_2).
+      apply Forall2_rev in Hq_1.
+      rewrite rev_involutive in Hq_1.
+      refine (let (d2,Hd2) := fifo_3q_deq_full q _ in _).
+      { intros H; rewrite H, Hp3, rev_app_distr in Hq_1.
+        inversion Hq_1. }
+      destruct d2 as (u,q1).
+      refine (let (d3,Hd3) := fifo_3q_deq_full q1 _ in _).
+      { intros H; rewrite Hd2, H, Hp3, Hp2 in Hq_1. 
+        repeat rewrite rev_app_distr in Hq_1.
+        inversion Hq_1. inversion H5. }
+      destruct d3 as (v,q2).
+      refine(let (q3,Hq3) := fifo_3q_enq_full q2 (node v y u) in  exist _ q3 _).
       rewrite Hp1, Hq3, rev_app_distr; simpl.
-      rewrite bft_f_fix_3; simpl; split; auto.
+      rewrite Hp3, Hp2, Hd2, Hd3 in Hq_1.
+      repeat rewrite rev_app_distr in Hq_1.
+      simpl in Hq_1.
+      apply Forall2_cons_inv in Hq_1; destruct Hq_1 as (Hq_3 & Hq_1).
+      apply Forall2_cons_inv in Hq_1; destruct Hq_1 as (Hq_4 & Hq_1).
+      apply Forall2_rev in Hq_1.
+      rewrite rev_involutive in Hq_1.
+      split; auto.
+      rewrite bft_f_fix_3; simpl; f_equal.
+      rewrite <- Hq_2, Hd2, Hd3; f_equal; simpl.
+      rewrite app_ass; auto.
   Defined.
+  
+  Section bfr.
 
-  Section bfn.
-
-    Let bfn_3q_full (t : bt X) : { t' | t ~t t' /\ is_seq_from 0 (bft_std t') }.
+    Let bfr_3q_full (t : bt X) (l : list Y) : m_bt t = length l -> { t' | t ~t t' /\ bft_std t' = l }.
     Proof.
-      refine (match @bfn_3q_f 0 (fifo_3q_enq fifo_3q_nil t) with 
+      intros H.
+      refine (match @bfr_3q_f (fifo_3q_enq fifo_3q_nil t) l _ with 
         | exist _ q Hq => let (d1,Hd1) := fifo_3q_deq_full q _ in _ 
       end).
-      all: cycle 1. (* We queue 1 PO *) 
-      revert Hd1; refine (match d1 with (x,q1) => fun Hq1 => exist _ x _ end); simpl in Hq1.
-      all: cycle 1. (* We queue 1 PO *) 
-
-      + intros H; rewrite fifo_3q_enq_spec, fifo_3q_nil_spec, H in Hq.
-        apply proj1 in Hq; inversion Hq.
-
-      + rewrite fifo_3q_enq_spec, fifo_3q_nil_spec in Hq; destruct Hq as (H1 & H2).
-        rewrite <- bft_std_eq_bft.
-        rewrite Hq1 in H1; simpl in H1.
-        apply Forall2_snoc_inv with (l := nil) in H1.
-        destruct H1 as (G1 & H1).
-        apply Forall2_nil_inv_right in H1.
-        apply f_equal with (f := @rev _) in H1.
-        rewrite rev_involutive in H1; simpl in H1.
-        rewrite Hq1, H1 in H2; simpl in H2.
-        auto.
+      { unfold fifo_3q_sum; rewrite fifo_3q_enq_spec, fifo_3q_nil_spec; simpl; omega. }
+      { intros E; rewrite E in Hq; apply proj2 in Hq; simpl in Hq.
+        rewrite bft_f_fix_0 in Hq; subst.
+        generalize (m_bt_ge_1 t); simpl in *; omega. }
+      destruct Hq as (Hq_1 & Hq_2).
+      destruct d1 as (t',q').
+      exists t'.
+      apply Forall2_rev in Hq_1.
+      rewrite fifo_3q_enq_spec, fifo_3q_nil_spec, rev_involutive, Hd1 in Hq_1; simpl in Hq_1.
+      apply Forall2_cons_inv in Hq_1.
+      destruct Hq_1 as (Hq_3 & Hq_1).
+      apply Forall2_nil_inv_right in Hq_1.
+      split; auto.
+      rewrite Hd1, Hq_1 in Hq_2.
+      simpl in Hq_2.
+      rewrite <- bft_std_eq_bft; auto.
     Qed.
 
-    Definition bfn_3q t := proj1_sig (bfn_3q_full t).
+    Definition bfr_3q t l H := proj1_sig (bfr_3q_full t l H).
 
-    Fact bfn_3q_spec_1 t : t ~t bfn_3q t.
-    Proof. apply (proj2_sig (bfn_3q_full t)). Qed.
+    Fact bfr_3q_spec_1 t l H : t ~t bfr_3q t l H.
+    Proof. apply (proj2_sig (bfr_3q_full t l H)). Qed.
 
-    Fact bfn_3q_spec_2 t : exists n, bft_std (bfn_3q t) = seq_an 0 n.
-    Proof. apply is_seq_from_spec, (proj2_sig (bfn_3q_full t)). Qed.
+    Fact bfr_3q_spec_2 t l H : bft_std (bfr_3q t l H) = l.
+    Proof. apply (proj2_sig (bfr_3q_full t l H)). Qed.
 
-  End bfn.
+  End bfr.
 
-End bfn.
+End bfr_3q.
 
 (* Notice that fifo_3q_deq is extracted to a function that loops forever
    if the input is the empty queue, ie does not following the spec *)
@@ -279,10 +139,10 @@ Extract Inductive bool => "bool" [ "true" "false" ].
 Extract Inductive prod => "(*)"  [ "(,)" ].
 Extract Inductive nat => int [ "0" "succ" ] "(fun fO fS n -> if n=0 then fO () else fS (n-1))".
 
-Recursive Extraction bfn_3q.
+Recursive Extraction bfr_3q.
 
-Check bfn_3q.
-Check bfn_3q_spec_1.
-Check bfn_3q_spec_2.
+Check bfr_3q.
+Check bfr_3q_spec_1.
+Check bfr_3q_spec_2.
              
 
